Use the [bytes] type added in coq-prelude

lib/Bytes.v
@@ -1,40 +1,14 @@
 From Coq Require Export Byte.
-From Prelude Require Import All.
+From Prelude Require Import All Bytes.
 From Comparse Require Import Monad Combinators.
 
 #[program]
-Instance byte_EquDec : EquDec byte :=
-  { equalb := Byte.eqb
-  }.
-
-Next Obligation.
-  split.
-  + apply Byte.byte_dec_lb.
-  + apply Byte.byte_dec_bl.
-Defined.
-
-Inductive bytes := to_bytes { of_bytes : list byte }.
-Definition id_byte (x : byte) := x.
-
-Declare Scope bytes_scope.
-Delimit Scope bytes_scope with bytes.
-Bind Scope bytes_scope with bytes.
-
-String Notation bytes to_bytes of_bytes : bytes_scope.
-String Notation byte id_byte id_byte : byte_scope.
-
-Definition append (x y : bytes) :=
-  to_bytes (List.app (of_bytes x) (of_bytes y)).
-
-Infix "++" := append : bytes_scope.
-
-#[program]
 Instance bytes_Input : Input bytes byte :=
-  { length := fun x => List.length (of_bytes x)
+  { length := fun x => List.length (unwrap_bytes x)
   ; unpack := fun (x : bytes) =>
                 match x with
-                | to_bytes [] => None
-                | to_bytes (x :: rst) => Some (x, to_bytes rst)
+                | wrap_bytes [] => None
+                | wrap_bytes (x :: rst) => Some (x, wrap_bytes rst)
                 end
   }.
 
@@ -50,7 +24,7 @@ Next Obligation.
   + split.
     ++ intros _.
        exists x.
-       exists (to_bytes rst).
+       exists (wrap_bytes rst).
        reflexivity.
     ++ intros _.
        apply PeanoNat.Nat.lt_0_succ.
